\documentclass{article}

\usepackage[margin=0.5in]{geometry}

\title{Problem Set 3}
\author{Mark Xavier (xaviem01)}

\begin{document}
	\maketitle
	
	\begin{enumerate}
		
		%% Problem 1
		\item Constraint 1: Any set $W_i \in W$ where $W_i$ is also in $Y$, the union of all such $W_i$ should include any atom of $U$ exactly once.  In other words, $\forall a \in U,$ if $a \in Y$ then it is only in $Y$ once. In the example given, we cannot have $Y=\{a,d,f,h\}, \{b,d,f,h\}$ as $f$ and $h$ are in $Y$ twice.
		
		Constraint 2: For the problem to actually be satisfiable, the union of all sets $W_i \in W$ must include every $a \in U$ \textbf{at least once}.  If this constraint is not met, the problem is unsatisfiable as no collection of $W_i$ will include every atom in $S$.  If, in the example given, $W$ did not include a single $W_i$ that included $a$, the problem would be unsolvable.
		
		Constraint 3: $\forall_{W_i} \in W, j \in W_i \Leftrightarrow j \in U$ - this is given via the problem prompt but is an additional constraint. 
		
		Constraint 4: This follows from constraint one, however $Y$ may not include any $W_i \in W$ more than once, so $Y$ cannot include $\{a,d,f,h\}$ twice.
		
		%% Problem 2
		\item Problem 2:
			
			\begin{enumerate}
				
				%% 2a
				\item {\tt Parent(Anne, Ted)}
				
				%% 2b
				\item $\forall_{x, y} \phantom{a} {\tt Parent(x, y) \Rightarrow Earlier(Birth(p), Birth(q))}$
				
				%% 2c
				\item $\forall_{p,q}, {\tt Living(p, t) \Leftrightarrow Earlier(Birth(p), t) \wedge Earlier(t, Death(p))}$
				
				%% 2d
				\item $\forall_{ta, tb} \phantom{a} {\tt Earlier(ta,tb) \Rightarrow \neg Earlier(tb,ta)}$ (I use implies instead of iff to account for the case where ta == tb)
				
				%% 2e
				\item $\forall_{ta,tb,tc} \phantom{a} {\tt Earlier(ta,tb) \wedge Earlier(tb, tc) \Rightarrow Earlier(ta, tc)}$
				
				%% 2f
				\item $\forall_p \phantom{a} \exists_t \phantom{a} {\tt s.t. Living(p,t)}$
				
				%% 2g
				\item ${\tt \neg Living(Ted, Born(Anne))}$
				
				%% 2h
				\item $\forall_p \phantom{a} {\tt Earlier(Born(p), Death(p))}$
				 
			\end{enumerate}
		
		%% Problem 3
		\item After conversion to CNF, we are left with the following clauses:
		
		a.\phantom{1} {\tt Parent(Anne, Ted)}\\
		b.\phantom{1} ${\tt \neg Parent(x,y) \vee Earlier(Birth(x), Birth(y))}$\\
		c1. ${\tt \neg Living(p,t) \vee Earlier(Birth(p), t)}$\\
		c2. ${\tt \neg Living(p,t) \vee Earlier(t, Death(p))}$\\
		c3. ${\tt \neg Earlier(Birth(p),t) \vee \neg Earlier(t, Death(p)) \vee Living(p,t)}$\\
		d.\phantom{1} ${\tt \neg Earlier(ta, tb) \vee \neg Earlier(tb, ta)}$\\
		S: {\tt Living(Ted, Born(Anne))} - \textbf{this is our negated assumption to prove.}
		
		The resolutions done follow below:
		
		\begin{tabular}{|c|c|c|c|}
			\hline
			ID & Clauses & Substitution & Resolution\\
			\hline
			r1 & a, b & $\{x \rightarrow Anne, y \rightarrow Ted\}$ & {\tt E(B(Anne), B(Ted))}\\
			\hline
			r2 & r1, d & $\{ta \rightarrow B(Anne), tb \rightarrow B(Ted)\}$ & ${\tt \neg E(B(Ted), B(Anne))}$\\
			\hline
			r3 & r2, c1 & $\{p \rightarrow Ted, t \rightarrow B(Anne)\}$ & ${\tt \neg L(Ted, B(Anne))}$\\
			\hline
			sol & r3, S & N/A & negation \\
			\hline
		\end{tabular}
		
		And we prove by contradiction that $S$ cannot be true.
		
		\pagebreak
		
		%% Problem 4
		\item After conversion to CNF, we are left with the following clauses:
		
		c1. ${\tt \neg Living(p,t) \vee Earlier(Birth(p), t)}$\\
		c2. ${\tt \neg Living(p,t) \vee Earlier(t, Death(p))}$\\
		c3. ${\tt \neg Earlier(Birth(p),t) \vee \neg Earlier(t, Death(p)) \vee Living(p,t)}$\\
		e.\phantom{1} ${\tt \neg Earlier(ta, tb) \vee \neg Earlier(tb, tc) \vee Earlier(ta, tc)}$\\
		f.\phantom{1} ${\tt Living(p, \lambda(p))}$\\
		S. ${\tt \neg Earlier(Born(p), Death(p))}$ - \textbf{this is our negated assumption to prove.}
		
		Again, the resolutions follow:
		
		\begin{tabular}{|c|c|c|c|}
			\hline
			ID & Clauses & Substitution & Resolution\\
			\hline
			r1 & c1, f & $\lambda(p) \rightarrow t$ & ${\tt E(B(p),t)}$\\
			\hline
			r2 & c2, f & $\lambda(p) \rightarrow t$ & ${\tt E(t,D(p))}$\\
			\hline
			r3 & r1, e & ${\tt ta \rightarrow B(p), tb \rightarrow t}$ & ${\tt \neg E(t, tc) \vee E(B(p),tc)}$\\
			\hline
			r4 & r2, r3 & ${\tt tc \rightarrow D(p)}$ & ${\tt E(B(p), D(P))}$\\
			\hline
			sol & r4, S & N/A & negation\\
			\hline
		\end{tabular}
	
		Hence we prove by contradiction that $S$ is not true.
		 
	\end{enumerate}
\end{document}